benchmark/proof/correct_calc_sum.v
@@ -8,6 +8,8 @@ From bpf.proof Require Import Clightlogic MatchState CorrectRel CommonLemma.
 
 From bpf.benchmark Require Import clightlogicexample BenchmarkTests.
 
+Locate nat_correct.
+
 (**
 unsigned int calc_sum(unsigned int v, unsigned int n)
 {
@@ -60,61 +62,205 @@ Section Calc_sum.
   (* [match_res] relates the Coq result and the C result *)
   Definition match_res : res -> val -> stateM -> Memory.Mem.mem -> Prop := fun x v st m => valu32_correct x v.
 
-  Instance correct_function3_calc_sum : correct_function3 p args res f fn (nil) true match_arg_list match_res.
+Ltac correct_body :=
+  intros st le m;
+(*  match type of a with
+  | DList.t _ ?A =>
+      unfold A in a
+  end;
+  car_cdr ;*)  unfold list_rel_arg,app;
+  match goal with
+    |- correct_body _ _ _ _ ?B _ ?INV
+                 _ _ _ _ =>
+      let I := fresh "INV" in
+      set (I := INV) ; simpl in I;
+      let B1 := eval simpl in B in
+        change B with B1
+  end.
+
+  Lemma calc_sum_eq :  forall n v,
+      calc_sum v n =
+        if Nat.eqb n 0 then returnM val32_zero
+        else bindM (get_add v val32_one) (fun nv : valu32_t => calc_sum nv (Nat.pred n)).
   Proof.
-    correct_function_from_body.
-    correct_body.
-    (** should we induction c0 before correct_body *)
-    unfold INV.
-    unfold f.
-    repeat intro.
-    get_invariant_more _v.
-    get_invariant_more _n.
+    destruct n.
+    - simpl. auto.
+    - intros.
+      simpl. reflexivity.
+  Qed.
 
-    unfold stateless, valu32_correct in H0.
-    unfold stateless, nat_correct in H2.
-    destruct H0 as (Hc_eq & (vi & Hvi_eq)).
-    subst c v.
-    simpl in c0.
-    (*generalize c0.*)
+  Ltac Zify.zify_post_hook ::= Z.div_mod_to_equations.
+
+  Lemma mod_eq : forall (x y:Z), (x >= 0 -> y > 0 -> x mod y = x -> x < y)%Z.
+  Proof.
+    intros.
+    zify.
+    intuition subst ; try lia.
+  Qed.
+
+
+
+  Instance correct_function3_calc_sum : forall a, correct_function3 p args res f fn (nil) true match_arg_list match_res a.
+  Proof.
+    intros. unfold args in a.
+    car_cdr.
+    revert c.
     induction c0.
-    {
-      simpl.
-      intros.
+    { intros.
+      correct_function_from_body.
+      correct_body.
+      repeat intro.
+      unfold INV in H.
+      get_invariant_more _v.
+      get_invariant_more _n.
+      unfold stateless, valu32_correct in H1.
+      unfold stateless, nat_correct in H3.
+      destruct H1 as (Hc_eq & (vi & Hvi_eq)).
+      destruct H3 as (H3 & _).
+      subst.
       eexists. exists m, Events.E0.
-      repeat split; unfold step2.
-      -
-        apply Smallstep.plus_star.
-        eapply Smallstep.plus_left'; eauto.
-        eapply step_ifthenelse.
-        econstructor; eauto.
-        econstructor; eauto.
-        Transparent Archi.ptr64.
-        econstructor; eauto.
+      repeat split.
+      + eapply Smallstep.star_step.
+        econstructor;eauto.
+        econstructor ; eauto.
+        econstructor;eauto.
+        econstructor ; eauto.
+        econstructor ; eauto.
+        simpl. reflexivity.
+        change (negb (Int.eq Int.one Int.zero)) with true.
         simpl.
-        unfold Cop.sem_cmp, Cop.sem_binarith, Cop.sem_cast; simpl.
-        rewrite <- H2. simpl.
+        eapply Smallstep.star_step.
+        econstructor;eauto.
+        econstructor ; eauto.
+        econstructor;eauto.
+        econstructor ; eauto.
+        econstructor ; eauto.
         reflexivity.
         reflexivity.
-
-        rewrite Int_eq_one_zero.
-        unfold negb.
-
-        forward_plus.
-        econstructor; eauto.
-        reflexivity.
-        reflexivity.
-        reflexivity.
-
-      - eexists.
-        unfold val32_zero; reflexivity.
-      - constructor.
-        reflexivity.
+      + eexists. reflexivity.
+      + econstructor;eauto.
     }
+    { intros.
+      correct_function_from_body.
+      correct_body.
+      unfold f. unfold app.
+      rewrite calc_sum_eq.
+      eapply correct_statement_if_body_expr.
+      simpl.
+      apply correct_statement_seq_set with (match_res1 := fun _ => stateless nat_correct c0).
+      +
+        intros.
+        unfold INV in H.
+        get_invariant_more _n.
+        unfold stateless,nat_correct in H0.
+        destruct H0 ; subst.
+        eexists.
+        repeat split.
+        econstructor;eauto.
+        econstructor;eauto. econstructor;eauto.
+        unfold Cop.sem_binary_operation.
+        unfold Cop.sem_sub. simpl.
+        unfold Cop.sem_binarith.
+        simpl. unfold Cop.sem_cast.
+        unfold Cop.classify_cast.
+        simpl.
+        {
+          destruct Archi.ptr64.
+          - repeat f_equal.
+            simpl.
+            simpl in H2.
+            unfold Int.sub.
+            rewrite H2. f_equal.
+            change (Int.unsigned (Int.repr 1))%Z with 1%Z.
+            lia.
+          - repeat f_equal.
+            simpl.
+            simpl in H2.
+            unfold Int.sub.
+            rewrite H2. f_equal.
+            change (Int.unsigned (Int.repr 1))%Z with 1%Z.
+            lia.
+        }
+        rewrite Int.unsigned_repr_eq.
+        apply Z.mod_small.
+        rewrite Int.unsigned_repr_eq in H2.
+        apply mod_eq in H2.
+        lia.
+        lia.
+        unfold Int.modulus.
+        reflexivity.
+        simpl.
+        constructor.
+        reflexivity.
+      + unfold INV.
+        simpl. intuition subst ; discriminate.
+      + intros.
+        eapply correct_statement_seq_body;eauto.
+        unfold typeof.
+        change (get_add c val32_one) with
+          (app (get_add: arrow_type (valu32_t :: valu32_t :: nil) (M valu32_t))
+                           (DList.DCons c
+                                                            (DList.DCons val32_one (DList.DNil _)))).
+        eapply correct_statement_call with (has_cast:=false).
+        reflexivity.
+        reflexivity.
+        reflexivity.
+        intros.
+        admit.
+        admit.
+        reflexivity.
+        reflexivity.
+        reflexivity.
+        unfold INV.
+        simpl. intuition subst ; discriminate.
+        simpl. intuition subst ; discriminate.
+        reflexivity.
+        instantiate (1:= true).
+        reflexivity.
+        admit.
+        intros.
+        unfold typeof.
+        change (calc_sum x0 c0) with
+          (app (calc_sum: arrow_type (valu32_t :: (nat:Type) :: nil) (M valu32_t))
+               (DList.DCons x0
+                            (DList.DCons c0 (DList.DNil _)))).
+        eapply correct_body_call_ret with (has_cast := false);eauto.
+        reflexivity.
+        reflexivity.
+        reflexivity.
+        admit.
+        admit.
+      +  simpl.
+        reflexivity.
+      + simpl.
+        intros. unfold INV in H.
+        get_invariant_more _n.
+        unfold stateless,nat_correct in H0.
+        intuition subst.
+        econstructor ; eauto.
+        econstructor ; eauto.
+        econstructor ; eauto.
+        simpl. unfold Cop.sem_cmp.
+        unfold Cop.classify_cmp.
+        simpl.
+        unfold Cop.sem_binarith.
+        simpl.
+        unfold Cop.sem_cast.
+        simpl.
+        destruct (Int.eq (Int.repr (Z.pos (Pos.of_succ_nat c0))) (Int.repr 0)) eqn:E; auto.
+        exfalso.
+        apply Int.same_if_eq in E.
+        apply (f_equal Int.unsigned) in E.
+        simpl in H3.
+        rewrite H3 in E.
+        change (Int.unsigned (Int.repr 0)) with 0%Z in E.
+        lia.
+        destruct Archi.ptr64.
+        simpl. rewrite E. reflexivity.
+        rewrite E. reflexivity.
+  Admitted.
 
-    simpl; simpl in IHc0.
-    unfold match_temp_env in H, IHc0.
-    
+
     (**r
       H2 :         Vint (Int.repr (Z.of_nat (S c0))) = v0
       Ihc0: ... -> Vint (Int.repr (Z.of_nat c0)) = v0 -> ...
